temp_commented_code.v
@@ -1,0 +1,286 @@
+(* Inductive LK : Node -> list prop -> list prop -> list prop -> list prop -> Prop :=
+(* Axiom : A |- A *)
+| LKA: forall p : prop, p +' [] ⇒ p +'' [] >< leaf
+(* Structral Rules *)
+(* Weakening *)
+|LKrW: forall G1 G2 D1 D2 (a: prop) n, G1 +' G2 ⇒ D1 +'' D2 >< n-> G1 +' G2 ⇒ a :: D1 +'' D2 >< onen n
+|LKlW: forall G1 G2 D1 D2 (a: prop) n, G1 +' G2 ⇒ D1 +'' D2 >< n -> a :: G1 +' G2  ⇒ D1 +'' D2 >< onen n
+(* Exchange *)
+|LKrE: forall G1 G2 D1 D2 (a b : prop) n, G1 +' G2 ⇒ (a :: b :: D1) +'' D2 >< n -> 
+        G1 +' G2 ⇒ (b :: a :: D1) +'' D2 >< onen n
+|LKlE: forall G1 G2 D1 D2 (a b : prop) n, (a :: b :: G1) +' G2 ⇒ D1 +'' D2 >< n ->
+        (b :: a :: G1) +' G2 ⇒ D1 +'' D2 >< onen n
+(* Contraction *)
+|LKrC: forall G1 G2 D1 D2 (a : prop) n, G1 +' G2 ⇒ (a :: a :: D1) +'' D2 >< n -> G1 +' G2 ⇒ (a :: D1) +'' D2 >< onen n
+|LKlC: forall G1 G2 D1 D2 (a : prop) n, a :: a :: G1 +' G2  ⇒ D1 +'' D2 >< n -> a :: G1 +' G2 ⇒ D1 +'' D2 >< onen n
+(* Logical Rules *)
+(* Conjunction *)
+|LKrA: forall G1 G2 D1 D2 (a b: prop) m n,
+G1 +' G2 ⇒ a :: D1 +'' D2 >< m-> G1 +' G2⇒ b :: D1 +'' D2 >< n -> G1 +' G2 ⇒ (a ∧ b) :: D1 +'' D2  >< twon m n
+|LKl1A: forall G1 G2 D1 D2 (a b : prop) n,
+a :: G1 +' G2 ⇒ D1 +'' D2 >< n -> (a ∧ b) :: G1 +' G2 ⇒ D1 +'' D2 >< onen n
+|LKl2A: forall G1 G2 D1 D2 (a b : prop) n,
+b :: G1 +' G2 ⇒ D1 +'' D2 >< n -> (a ∧ b) :: G1 +' G2 ⇒ D1 +'' D2 >< onen n
+(* Disjunction *)
+|LKr1O: forall G1 G2 D1 D2 (a b : prop) n,
+G1 +' G2 ⇒ a :: D1 +'' D2 >< n -> G1 +' G2 ⇒ (a ∨ b) :: D1 +'' D2 >< onen n
+|LKr2O: forall G1 G2 D1 D2 (a b : prop) n,
+G1 +' G2 ⇒ b :: D1 +'' D2 >< n -> G1 +' G2 ⇒ (a ∨ b) :: D1 +'' D2 >< onen n
+|LKlO: forall G1 G2 D1 D2 (a b : prop) m n,
+a :: G1 +' G2 ⇒ D1 +'' D2 >< m -> b :: G1 +' G2 ⇒ D1 +'' D2 >< n -> (a ∨ b) :: G1 +' G2  ⇒ D1 +'' D2 >< twon m n
+(* Negation *)
+|LKrN: forall G1 G2 D1 D2 (a : prop) n, a :: G1 +' G2 ⇒ D1 +'' D2 >< n -> G1 +' G2 ⇒ (¬ a) :: D1 +'' D2 >< onen n
+|LKlN: forall G1 G2 D1 D2 (a : prop) n, G1 +' G2 ⇒ a :: D1 +'' D2 >< n -> (¬ a) :: G1 +' G2  ⇒ D1 +'' D2 >< onen n
+(* Implication *)
+|LKrI: forall G1 G2 D1 D2 (a b : prop) n, a :: G1 +' G2  ⇒ b :: D1 +'' D2 >< n ->
+        G1 +' G2 ⇒ (a ⊃ b) :: D1 +'' D2 >< onen n
+|LKlI: forall G1 G2 D1 D2 (a b : prop) m n,
+        G1 +' G2 ⇒ a :: D1 +'' D2 >< m -> b :: G1 +' G2 ⇒ D1 +'' D2 >< n->
+        (a ⊃ b) :: G1 +' G2 ⇒ D1 +'' D2 >< twon m n
+where "G1 +' G2 ⇒ D1 +'' D2 >< n" := (LK n G1 G2 D1 D2). *)
+
+
+
+
+(* Theorem LK_Interpol_strong: forall n (G1 G2 D1 D2 : list prop),
+G1 ++ G2 ⇒ D1 ++ D2 >< n -> 
+(exists (c : prop) m1 m2, G1 ⇒ c :: D1 >< m1 /\ c :: G2 ⇒ D2 >< m2
+(* /\ lil (atom_lista c) (list_intersect (atom_list(G1 ++ G2)) (atom_list(D1 ++ D2)))). *)
+(* /\ (forall (x : atom), (In_prop x c) -> ((In_list_prop x (G1 ++ G2) /\ In_list_prop x (D1 ++ D2))))). *)
+/\ (atoms_of c) ⊆ ( (atoms_of_list (G1 ++ G2)) ∩ (atoms_of_list (D1 ++ D2)))).
+
+ induction n; intros G1 G2 D1 D2 H; inversion H.
+    -  destruct G1, G2, D1, D2; try discriminate; simpl in *; inversion H0; inversion H1; subst; try (rewrite app_nil_r in *).
+        + exists (p1 ∨ ¬ p1), (☉ (☉ (☉ (☉ (☉ leaf))))), (☉ leaf). repeat split.
+            * constructor 6. constructor 11. 
+            apply (LKrE [] [] [] (p1 ∨ ¬ p1) (p1) (☉ (☉ leaf))). simpl.
+            constructor 12. constructor 14. constructor 1.
+            * constructor 3. constructor 1.
+            * simpl. rewrite union_idr. 
+            rewrite union_refl. rewrite intersection_refl.
+            apply incl_reflexive.
+        + subst.
+        exists (¬ p1), (☉ leaf), (☉ leaf). repeat split.
+            * constructor 14. apply H.
+            * constructor 15. apply H.
+            * simpl. rewrite union_idr. rewrite intersection_refl.
+            apply incl_reflexive.
+        + destruct D1; inversion H6.
+        + subst. exists p1, leaf, leaf. repeat split.
+            * constructor 1.
+            * constructor 1.
+            * rewrite union_idr. rewrite intersection_refl.
+            apply incl_reflexive.
+        + subst; simpl in *.
+        exists (p1 ∧ ¬ p1), (☉ leaf), (☉ (☉ (☉ (☉ (☉ leaf))))). repeat split.
+            * constructor 2. constructor 1.
+            * constructor 7. constructor 9.
+            apply (LKlE [] [] [] (p1 ∧ ¬ p1) (p1) (☉ (☉ leaf))). simpl.
+            constructor 10. constructor 15. constructor 1.
+            * simpl. rewrite union_idr. 
+            rewrite union_refl. rewrite intersection_refl.
+            apply incl_reflexive.
+        + destruct D1; inversion H6.
+        + destruct G1; inversion H4.
+        + destruct G1; inversion H4.
+        + destruct G1; inversion H4.
+    - destruct D1, D2; simpl in *; try discriminate; try inversion H1; subst; simpl in *.
+        + rewrite <- app_nil_l in H3.
+        specialize (IHn G1 G2 [] (D2) H3) as H'.
+        destruct H' as [c [m1 [m2 [IH1 [IH2 IH3]]]]].
+        exists c, m1, (☉ m2). repeat split.
+            * apply IH1.
+            * constructor 2. apply IH2.
+            * apply incl_union_inter_absorb. simpl in IH3. auto.
+        + specialize (IHn G1 G2 D1 [] H3) as H'.
+        destruct H' as [c [m1 [m2 [IH1 [IH2 IH3]]]]].
+        exists c, (☉ (☉ m1)), m2. repeat split.
+            * apply (LKrE G1 [] D1 p c (☉ m1)). simpl.
+            constructor 2. apply IH1.
+            * apply IH2.
+            * apply incl_union_inter_absorb. auto.
+        + specialize (IHn G1 G2 D1 (p0 :: D2) H3) as H'.
+        destruct H' as [c [m1 [m2 [IH1 [IH2 IH3]]]]].
+        exists c, (☉ (☉ m1)), m2. repeat split.
+            * apply (LKrE G1 [] D1 p c (☉ m1)).
+            constructor 2. apply IH1.
+            * apply IH2.
+            * apply incl_union_inter_absorb. auto.
+    - destruct G1, G2; simpl in *; try discriminate; try inversion H1; subst; simpl in *. 
+        + specialize (IHn [] G2 D1 (D2) H2) as H'.
+        destruct H' as [c [m1 [m2 [IH1 [IH2 IH3]]]]].
+        exists c, m1, (☉ (☉ m2)). repeat split.
+            * apply IH1.
+            * apply (LKlE [] G2 D2 p c (☉ m2)). simpl.
+            constructor 3. apply IH2.
+            * apply incl_union_absorb_inter. auto.
+        + specialize (IHn G1 [] D1 (D2) H2) as H'.
+        destruct H' as [c [m1 [m2 [IH1 [IH2 IH3]]]]].
+        exists c, (☉ m1), m2. repeat split.
+            * constructor 3. apply IH1.
+            * apply IH2.
+            * apply incl_union_absorb_inter. auto.
+        + specialize (IHn G1 (p0 :: G2) D1 D2 H2) as H'.
+        destruct H' as [c [m1 [m2 [IH1 [IH2 IH3]]]]].
+        exists c, (☉ m1), m2. repeat split.
+            * constructor 3. apply IH1.
+            * apply IH2.
+            * apply incl_union_absorb_inter. auto.
+    - apply exchg_partition in H1. 
+    destruct H1 as [[H1 H1'] | [[D3 [H1 H1']] | [[H1 H1'] | [[H1 H1']| [[H1 H1'] | [[D3 [H1 H1']] | [H1 H1'] ]]]]]].
+        --  
+        specialize (IHn G1 G2 [] (D ++ a :: b :: D') H3) as H'.
+        destruct H' as [c [m1 [m2 [H6 [H6' H7]]]]].
+        exists c,m1 ,(☉ m2). repeat split.
+            + subst. apply H6.
+            + subst. constructor  4. apply H6'.
+            + simpl. rewrite (atoms_list_app D (b :: a :: D')).
+            simpl. rewrite (union_assoc (^V b) (^V a) (atoms_of_list D')).
+            rewrite (union_comm (^V b) (^V a) ).
+            simpl in H7. rewrite (atoms_list_app D (a :: b :: D')) in H7. 
+            simpl in H7. rewrite (union_assoc (^V a) (^V b) (atoms_of_list D')) in H7. apply H7.
+        -- rewrite H1' in H3. rewrite <- app_assoc in H3.
+        specialize (IHn G1 G2 D1 (D3 ++ a :: b :: D') H3) as H'.
+        destruct H' as [c [m1 [m2 [H6 [H6' H7]]]]].
+        exists c, m1, (☉ m2). repeat split.
+            + apply H6.
+            + rewrite H1. constructor 4. apply H6'.
+            + rewrite (atoms_list_app D (b :: a :: D')). 
+            rewrite H1'. rewrite (atoms_list_app D1 D3).
+            rewrite <- union_assoc. simpl. rewrite (union_assoc (^V b) (^V a) (atoms_of_list D')).
+            rewrite (union_comm (^V b) (^V a) ).
+            rewrite (atoms_list_app D1  (D3 ++ a :: b :: D')) in H7.
+            rewrite (atoms_list_app D3 (a :: b :: D')) in H7. 
+            simpl in H7. rewrite (union_assoc (^V a) (^V b) (atoms_of_list D')) in H7. apply H7.
+        --
+        specialize (IHn G1 G2 D (a :: b :: D') H3) as H'.
+        destruct H' as [c [m1 [m2 [H6 [H6' H7]]]]].
+        exists c, m1, (☉ m2). repeat split.
+            + rewrite H1. apply H6.
+            + rewrite H1'. rewrite <- app_nil_l. constructor 4. simpl. apply H6'.
+            + admit.
+        -- rewrite app_cons in H3. rewrite app_cons in H3. 
+        rewrite app_assoc in H3. rewrite app_assoc in H3. rewrite <- (app_assoc D [a] [b]) in H3.
+        specialize (IHn G1 G2 (D ++ [a] ++ [b]) (D') H3) as H'.
+        destruct H' as [c [m1 [m2 [H6 [H6' H7]]]]].
+        rewrite app_comm_cons in H6.
+        apply LKr_partition_mid_l in H6. destruct H6 as [m' H6].
+        rewrite app_assoc in H6. rewrite (app_cons [a] D c) in H6.
+        rewrite <- app_assoc in H6.
+        simpl in H6.
+        apply (LKr2O G1 (c :: D ++ [b]) c a m') in H6.
+        apply (LKrE G1 [] (D ++ [b]) (c ∨ a) c (☉ m')) in H6.
+        simpl in H6.
+        apply (LKr1O G1 (c ∨ a :: D ++ [b]) c a (☉ (☉ m'))) in H6.
+        apply (LKrC G1 (D ++ [b]) (c ∨ a) (☉ (☉ (☉ m')))) in H6.
+
+        specialize (LKA a) as H6''.
+        specialize (LKl_app_list [a] G2 [a] leaf H6'') as H8.
+        destruct H8 as [m3 H8].
+        apply LKl_cons_app in H8. destruct H8 as [m'' H8].
+
+        apply (LKrW (c :: G2) (D') a m2) in H6'.
+        apply (LKr_app_list ([a] ++ G2) [a] D' m'') in H8.
+        destruct H8 as [m4 H8]. apply (LK_cons_app ([a] ++ G2) [a] D' m4) in H8.
+        destruct H8 as [m5 H8]. simpl in H8.
+        specialize (LKlO G2 (a :: D') c a (☉ m2) m5 H6' H8) as H9.
+        exists (c ∨ a) , (☉ (☉ (☉ (☉ m')))), (☉ m2 ≍ m5). 
+        repeat split.
+            + rewrite H1. apply H6.
+            + rewrite H1'. apply H9.
+            + simpl. admit.
+            (* rewrite exchg_atoms_of_list.
+            replace (D ++ a :: b :: D') with ((D ++ [a] ++ [b]) ++
+            D').
+            apply H7. *)
+        -- replace (D ++ a :: b :: D') with ((D ++ a :: b) ++ D') in H3. 
+        specialize (IHn G1 G2 (D ++ a :: b) (D') H3) as H'.
+        destruct H' as [c [m1 [m2 [H6 [H6' H7]]]]].
+        exists c, (☉ m1), m2. repeat split.
+            + rewrite H1. apply (LKrE G1 (c::D) [] a b m1). simpl. apply H6.
+            + rewrite H1'. apply H6'.
+            + rewrite exchg_atoms_of_list. 
+            rewrite <- app_assoc in H7. simpl in H7. auto.
+            + rewrite <- app_assoc. simpl. reflexivity.
+        -- rewrite H1' in H3. rewrite app_comm_cons in H3. rewrite app_comm_cons in H3. rewrite app_assoc in H3.
+        specialize (IHn G1 G2 (D ++ a :: b :: D3) (D2) H3) as H'.
+        destruct H' as [c [m1 [m2 [H6 [H6' H7]]]]].
+        exists c, (☉ m1), m2. repeat split.
+            + subst. apply (LKrE G1 (c::D) D3 a b m1). simpl. apply H6.
+            +subst. apply H6'.
+            + rewrite exchg_atoms_of_list.
+            replace ((D ++ a :: b :: D3) ++ D2) with (D ++ a :: b :: D') in H7.
+            auto.
+            {rewrite <- app_assoc. simpl. rewrite H1'. reflexivity. }
+        -- rewrite <- app_nil_r in H3.
+        specialize (IHn G1 G2 (D ++ a :: b :: D') [] H3) as H'.
+        destruct H' as [c [m1 [m2 [H6 [H6' H7]]]]].
+        exists c, (☉ m1), m2. repeat split.
+            + subst. apply (LKrE G1 (c::D) D' a b m1). apply H6.
+            + subst. apply H6'.
+            + rewrite exchg_atoms_of_list. rewrite app_nil_r in H7.
+            auto.
+    - admit.
+    -admit.
+    - admit.
+    - admit.
+    - admit.
+    - admit.
+    - admit.
+    - admit.
+    - admit.
+    - admit.
+    - subst. destruct D1, D2; inversion H2; subst.
+        + specialize (IHn1 G1 G2 [] (a :: D2) H4) as H6. destruct H6 as [c0 [m1 [m2 [H6 [H6' H7]]]]].
+        specialize  (IHn2 G1 G2 [] (b :: D2) H5) as H8. destruct H8 as [c1 [m1' [m2' [H8 [H8' H9]]]]].
+        exists (c0 ∧ c1), ( m1 ≍ m1'), ( (☉ m2) ≍ (☉ m2')). repeat split.
+            * constructor 8. apply H6. apply H8.
+            * constructor 8.
+                ** constructor 9. apply H6'.
+                ** constructor 10. apply H8'.
+            * simpl. simpl in H9. simpl in H7.
+            apply (incl_union_inter_add).
+                ** apply H7.
+                ** apply H9.
+        + simpl in *. 
+        specialize (IHn1 G1 G2 (a :: D1) [] H4) as H6. destruct H6 as [c0 [m1 [m2 [H6 [H6' H7]]]]].
+        specialize  (IHn2 G1 G2 (b :: D1) [] H5) as H8. destruct H8 as [c1 [m1' [m2' [H8 [H8' H9]]]]].
+        exists (c0 ∨ c1), 
+        (☉ ((☉ ☉ m1) ≍ (☉ ☉ m1'))),
+        (m2 ≍ m2'). repeat split.
+            * apply (LKrE G1 [] D1 (a ∧ b) (c0 ∨ c1) ((☉ ☉ m1) ≍ (☉ ☉ m1'))).
+            simpl. constructor 8.
+                ** apply (LKrE G1 [] D1 (c0 ∨ c1) (a) (☉ m1)).
+                simpl. constructor 11. apply H6.
+                ** apply (LKrE G1 [] D1 (c0 ∨ c1) (b) (☉ m1')).
+                simpl. constructor 12. apply H8.
+            * constructor 13.
+                ** apply H6'.
+                ** apply H8'.
+            * simpl. simpl in H9. simpl in H7.
+            apply (incl_union_inter_add).
+                ** apply H7.
+                ** apply H9.
+        + simpl in *. 
+        specialize (IHn1 G1 G2 (a :: D1) (p0 :: D2 ) H4) as H6. destruct H6 as [c0 [m1 [m2 [H6 [H6' H7]]]]].
+        specialize  (IHn2 G1 G2 (b :: D1) (p0 :: D2 ) H5) as H8. destruct H8 as [c1 [m1' [m2' [H8 [H8' H9]]]]].
+        exists (c0 ∨ c1), 
+        (☉ ((☉ ☉ m1) ≍ (☉ ☉ m1'))),
+        (m2 ≍ m2'). repeat split.
+            * apply (LKrE G1 [] D1 (a ∧ b) (c0 ∨ c1) ((☉ ☉ m1) ≍ (☉ ☉ m1'))).
+            simpl. constructor 8.
+                ** apply (LKrE G1 [] D1 (c0 ∨ c1) (a) (☉ m1)).
+                simpl. constructor 11. apply H6.
+                ** apply (LKrE G1 [] D1 (c0 ∨ c1) (b) (☉ m1')).
+                simpl. constructor 12. apply H8.
+            * constructor 13.
+                ** apply H6'.
+                ** apply H8'.
+            * simpl. simpl in H9. simpl in H7.
+            apply (incl_union_inter_add).
+                ** apply H7.
+                ** apply H9.
+    - admit.
+    - admit.
+
+Admitted. *)
